iris/UkRunSys.v
@@ -527,12 +527,12 @@ Section UkRunSys.
   Proof.
     intros Hn Hexit Hfork Hexec Hsbrk H3 H4 H5 H8 Hcl Hdp Hop Hcd Hal4.
     iIntros "#Hi Hrun Hsb Hcont".
-    iDestruct "Hrun" as (xi C pt Rfd Rut sz M pm fdv cw gn cs pidv) "(%Hlo & %Hpm & %HRut & Hheap & Hstk & Hufd & Hcwda & Hcha & #Hmy & Hpayv & #Hdep & Hb)".
+    iDestruct "Hrun" as (xi C pt Rfd Rut sz M pm fdv cw gn cs pidv) "(%Hlo & %Hpm & %Hlzf & %HRut & Hheap & Hstk & Hufd & Hcwda & Hcha & #Hmy & Hpayv & #Hdep & Hb)".
     iMod (udepw_mint N m pc _ M pm _ fdv cw gn cs pidv
                 with "Hdep Hmy Hsb Hheap Hufd") as "(Hheap & Hufd & Hdepn)".
     iDestruct (uinstr_is_uk_instr with "Hheap Hi") as %Hui.
     iDestruct (uvb_x0 with "Hb") as "[%Hx0 Hb]".
-    iApply (UkStep.wp_uk_ecall C pt Rfd Rut pm sz Hlo Hpm HRut M m pc fdv cw gn cs pidv Hui
+    iApply (UkStep.wp_uk_ecall C pt Rfd Rut pm sz Hlo Hpm HRut Hlzf M m pc fdv cw gn cs pidv Hui
               (fun (s : mstate)
                    (Hp : register_lookup cur_privilege s.(sregs) = User)
                    (Hc : register_lookup (R_bitvector_64 PC) s.(sregs) = pc) =>
@@ -668,14 +668,14 @@ Section UkRunSys.
   Proof.
     intros Hn Hal4.
     iIntros "#Hi Hrun Hsb Hcwd Hcont".
-    iDestruct "Hrun" as (xi C pt Rfd Rut sz M pm fdv cw gn cs pidv) "(%Hlo & %Hpm & %HRut & Hheap & Hstk & Hufd & Hcwda & Hcha & #Hmy & Hpayv & #Hdep & Hb)".
+    iDestruct "Hrun" as (xi C pt Rfd Rut sz M pm fdv cw gn cs pidv) "(%Hlo & %Hpm & %Hlzf & %HRut & Hheap & Hstk & Hufd & Hcwda & Hcha & #Hmy & Hpayv & #Hdep & Hb)".
     (* the key's cwd IS the one the caller's half is at *)
     iDestruct (ucwd_agree with "Hcwda Hcwd") as %->.
     iMod (udepw_mint N m pc _ M pm _ fdv c gn cs pidv
                 with "Hdep Hmy Hsb Hheap Hufd") as "(Hheap & Hufd & Hdepn)".
     iDestruct (uinstr_is_uk_instr with "Hheap Hi") as %Hui.
     iDestruct (uvb_x0 with "Hb") as "[%Hx0 Hb]".
-    iApply (UkStep.wp_uk_ecall C pt Rfd Rut pm sz Hlo Hpm HRut M m pc fdv c gn cs pidv Hui
+    iApply (UkStep.wp_uk_ecall C pt Rfd Rut pm sz Hlo Hpm HRut Hlzf M m pc fdv c gn cs pidv Hui
               (fun (s : mstate)
                    (Hp : register_lookup cur_privilege s.(sregs) = User)
                    (Hc : register_lookup (R_bitvector_64 PC) s.(sregs) = pc) =>
@@ -834,12 +834,12 @@ Section UkRunSys.
   Proof.
     intros Hn Hal4.
     iIntros "#Hi Hrun Hsb Hstd Hcont".
-    iDestruct "Hrun" as (xi C pt Rfd Rut sz M pm fdv cw gn cs pidv) "(%Hlo & %Hpm & %HRut & Hheap & Hstk & Hufd & Hcwda & Hcha & #Hmy & Hpayv & #Hdep & Hb)".
+    iDestruct "Hrun" as (xi C pt Rfd Rut sz M pm fdv cw gn cs pidv) "(%Hlo & %Hpm & %Hlzf & %HRut & Hheap & Hstk & Hufd & Hcwda & Hcha & #Hmy & Hpayv & #Hdep & Hb)".
     iMod (udepw_mint N m pc _ M pm _ fdv cw gn cs pidv
                 with "Hdep Hmy Hsb Hheap Hufd") as "(Hheap & Hufd & Hdepn)".
     iDestruct (uinstr_is_uk_instr with "Hheap Hi") as %Hui.
     iDestruct (uvb_x0 with "Hb") as "[%Hx0 Hb]".
-    iApply (UkStep.wp_uk_ecall C pt Rfd Rut pm sz Hlo Hpm HRut M m pc fdv cw gn cs pidv Hui
+    iApply (UkStep.wp_uk_ecall C pt Rfd Rut pm sz Hlo Hpm HRut Hlzf M m pc fdv cw gn cs pidv Hui
               (fun (s : mstate)
                    (Hp : register_lookup cur_privilege s.(sregs) = User)
                    (Hc : register_lookup (R_bitvector_64 PC) s.(sregs) = pc) =>
@@ -989,7 +989,7 @@ Section UkRunSys.
   Proof.
     intros Hn Harg Hstne Hal4.
     iIntros "#Hi Hrun Hsb Hstd Hh0 Hcont".
-    iDestruct "Hrun" as (xi C pt Rfd Rut sz M pm fdv cw gn cs pidv) "(%Hlo & %Hpm & %HRut & Hheap & Hstk & Hufd & Hcwda & Hcha & #Hmy & Hpayv & #Hdep & Hb)".
+    iDestruct "Hrun" as (xi C pt Rfd Rut sz M pm fdv cw gn cs pidv) "(%Hlo & %Hpm & %Hlzf & %HRut & Hheap & Hstk & Hufd & Hcwda & Hcha & #Hmy & Hpayv & #Hdep & Hb)".
     iMod (udepw_mint N m pc _ M pm _ fdv cw gn cs pidv
                 with "Hdep Hmy Hsb Hheap Hufd") as "(Hheap & Hufd & Hdepn)".
     iDestruct (uinstr_is_uk_instr with "Hheap Hi") as %Hui.
@@ -1001,7 +1001,7 @@ Section UkRunSys.
     (* ...and the slot the copy lands in is never the source's, which is
        what lets the claim come back at the ledger the copy left *)
     iDestruct (ufd_own_ne_lowest (ukn_fd N) l fd0 st Hstne with "Hstd Hh0") as %Hnel.
-    iApply (UkStep.wp_uk_ecall C pt Rfd Rut pm sz Hlo Hpm HRut M m pc fdv cw gn cs pidv Hui
+    iApply (UkStep.wp_uk_ecall C pt Rfd Rut pm sz Hlo Hpm HRut Hlzf M m pc fdv cw gn cs pidv Hui
               (fun (s : mstate)
                    (Hp : register_lookup cur_privilege s.(sregs) = User)
                    (Hc : register_lookup (R_bitvector_64 PC) s.(sregs) = pc) =>
@@ -1139,12 +1139,12 @@ Section UkRunSys.
   Proof.
     intros Hn Hal4.
     iIntros "#Hi Hrun Hsb Hstd Hcont".
-    iDestruct "Hrun" as (xi C pt Rfd Rut sz M pm fdv cw gn cs pidv) "(%Hlo & %Hpm & %HRut & Hheap & Hstk & Hufd & Hcwda & Hcha & #Hmy & Hpayv & #Hdep & Hb)".
+    iDestruct "Hrun" as (xi C pt Rfd Rut sz M pm fdv cw gn cs pidv) "(%Hlo & %Hpm & %Hlzf & %HRut & Hheap & Hstk & Hufd & Hcwda & Hcha & #Hmy & Hpayv & #Hdep & Hb)".
     iMod (udepw_mint N m pc _ M pm _ fdv cw gn cs pidv
                 with "Hdep Hmy Hsb Hheap Hufd") as "(Hheap & Hufd & Hdepn)".
     iDestruct (uinstr_is_uk_instr with "Hheap Hi") as %Hui.
     iDestruct (uvb_x0 with "Hb") as "[%Hx0 Hb]".
-    iApply (UkStep.wp_uk_ecall C pt Rfd Rut pm sz Hlo Hpm HRut M m pc fdv cw gn cs pidv Hui
+    iApply (UkStep.wp_uk_ecall C pt Rfd Rut pm sz Hlo Hpm HRut Hlzf M m pc fdv cw gn cs pidv Hui
               (fun (s : mstate)
                    (Hp : register_lookup cur_privilege s.(sregs) = User)
                    (Hc : register_lookup (R_bitvector_64 PC) s.(sregs) = pc) =>
@@ -1303,7 +1303,7 @@ Section UkRunSys.
   Proof.
     intros Hn Harg Hlt Hrow Hal4.
     iIntros "#Hi Hrun Hsb Hstd Hcont".
-    iDestruct "Hrun" as (xi C pt Rfd Rut sz M pm fdv cw gn cs pidv) "(%Hlo & %Hpm & %HRut & Hheap & Hstk & Hufd & Hcwda & Hcha & #Hmy & Hpayv & #Hdep & Hb)".
+    iDestruct "Hrun" as (xi C pt Rfd Rut sz M pm fdv cw gn cs pidv) "(%Hlo & %Hpm & %Hlzf & %HRut & Hheap & Hstk & Hufd & Hcwda & Hcha & #Hmy & Hpayv & #Hdep & Hb)".
     (* THE LEDGER READS THE VIEW, which is the whole argument: the source
        slot is CLOSED in the table, so dup's success arm copies [FdClosed]
        into a slot the scan already found closed and the list does not
@@ -1316,7 +1316,7 @@ Section UkRunSys.
                 with "Hdep Hmy Hsb Hheap Hufd") as "(Hheap & Hufd & Hdepn)".
     iDestruct (uinstr_is_uk_instr with "Hheap Hi") as %Hui.
     iDestruct (uvb_x0 with "Hb") as "[%Hx0 Hb]".
-    iApply (UkStep.wp_uk_ecall C pt Rfd Rut pm sz Hlo Hpm HRut M m pc fdv cw gn cs pidv Hui
+    iApply (UkStep.wp_uk_ecall C pt Rfd Rut pm sz Hlo Hpm HRut Hlzf M m pc fdv cw gn cs pidv Hui
               (fun (s : mstate)
                    (Hp : register_lookup cur_privilege s.(sregs) = User)
                    (Hc : register_lookup (R_bitvector_64 PC) s.(sregs) = pc) =>
@@ -1462,14 +1462,14 @@ Section UkRunSys.
   Proof.
     intros Hn Harg Hal4.
     iIntros "#Hi Hrun Hsb Hh Hcont".
-    iDestruct "Hrun" as (xi C pt Rfd Rut sz M pm fdv cw gn cs pidv) "(%Hlo & %Hpm & %HRut & Hheap & Hstk & Hufd & Hcwda & Hcha & #Hmy & Hpayv & #Hdep & Hb)".
+    iDestruct "Hrun" as (xi C pt Rfd Rut sz M pm fdv cw gn cs pidv) "(%Hlo & %Hpm & %Hlzf & %HRut & Hheap & Hstk & Hufd & Hcwda & Hcha & #Hmy & Hpayv & #Hdep & Hb)".
     iMod (udepw_mint N m pc _ M pm _ fdv cw gn cs pidv
                 with "Hdep Hmy Hsb Hheap Hufd") as "(Hheap & Hufd & Hdepn)".
     iDestruct (uinstr_is_uk_instr with "Hheap Hi") as %Hui.
     iDestruct (uvb_x0 with "Hb") as "[%Hx0 Hb]".
     iDestruct (ufd_agree with "Hufd Hh") as %Hi.
     iDestruct (ufd_ne with "Hh") as %Hne.
-    iApply (UkStep.wp_uk_ecall C pt Rfd Rut pm sz Hlo Hpm HRut M m pc fdv cw gn cs pidv Hui
+    iApply (UkStep.wp_uk_ecall C pt Rfd Rut pm sz Hlo Hpm HRut Hlzf M m pc fdv cw gn cs pidv Hui
               (fun (s : mstate)
                    (Hp : register_lookup cur_privilege s.(sregs) = User)
                    (Hc : register_lookup (R_bitvector_64 PC) s.(sregs) = pc) =>
@@ -1574,7 +1574,7 @@ Section UkRunSys.
   Proof.
     intros Hn Harg Hs Hkl Hne Hal4.
     iIntros "#Hi Hrun Hsb Hstd Hcont".
-    iDestruct "Hrun" as (xi C pt Rfd Rut sz M pm fdv cw gn cs pidv) "(%Hlo & %Hpm & %HRut & Hheap & Hstk & Hufd & Hcwda & Hcha & #Hmy & Hpayv & #Hdep & Hb)".
+    iDestruct "Hrun" as (xi C pt Rfd Rut sz M pm fdv cw gn cs pidv) "(%Hlo & %Hpm & %Hlzf & %HRut & Hheap & Hstk & Hufd & Hcwda & Hcha & #Hmy & Hpayv & #Hdep & Hb)".
     iMod (udepw_mint N m pc _ M pm _ fdv cw gn cs pidv
                 with "Hdep Hmy Hsb Hheap Hufd") as "(Hheap & Hufd & Hdepn)".
     iDestruct (uinstr_is_uk_instr with "Hheap Hi") as %Hui.
@@ -1582,7 +1582,7 @@ Section UkRunSys.
     iDestruct (ustd_agree with "Hufd Hstd") as %Hst.
     assert (Hi : fdv !! fd = Some st).
     { rewrite <- (lookup_take fdv NSTD fd Hs). by rewrite Hst. }
-    iApply (UkStep.wp_uk_ecall C pt Rfd Rut pm sz Hlo Hpm HRut M m pc fdv cw gn cs pidv Hui
+    iApply (UkStep.wp_uk_ecall C pt Rfd Rut pm sz Hlo Hpm HRut Hlzf M m pc fdv cw gn cs pidv Hui
               (fun (s : mstate)
                    (Hp : register_lookup cur_privilege s.(sregs) = User)
                    (Hc : register_lookup (R_bitvector_64 PC) s.(sregs) = pc) =>
@@ -1705,14 +1705,14 @@ Section UkRunSys.
   Proof.
     intros Hn Ha1 Hcnt Hal4.
     iIntros "#Hi Hbs Hrun Hsb Hcont".
-    iDestruct "Hrun" as (xi C pt Rfd Rut sz M pm fdv cw gn cs pidv) "(%Hlo & %Hpm & %HRut & Hheap & Hstk & Hufd & Hcwda & Hcha & #Hmy & Hpayv & #Hdep & Hb)".
+    iDestruct "Hrun" as (xi C pt Rfd Rut sz M pm fdv cw gn cs pidv) "(%Hlo & %Hpm & %Hlzf & %HRut & Hheap & Hstk & Hufd & Hcwda & Hcha & #Hmy & Hpayv & #Hdep & Hb)".
     iMod (udepw_mint N m pc _ M pm _ fdv cw gn cs pidv
                 with "Hdep Hmy Hsb Hheap Hufd") as "(Hheap & Hufd & Hdepn)".
     iDestruct (uinstr_is_uk_instr with "Hheap Hi") as %Hui.
     iDestruct (uvb_x0 with "Hb") as "[%Hx0 Hb]".
     (* the run is in the image, and does not wrap *)
     iDestruct (uheap_ubytes_img with "Hheap Hbs") as %Himg.
-    iApply (UkStep.wp_uk_ecall C pt Rfd Rut pm sz Hlo Hpm HRut M m pc fdv cw gn cs pidv Hui
+    iApply (UkStep.wp_uk_ecall C pt Rfd Rut pm sz Hlo Hpm HRut Hlzf M m pc fdv cw gn cs pidv Hui
               (fun (s : mstate)
                    (Hp : register_lookup cur_privilege s.(sregs) = User)
                    (Hc : register_lookup (R_bitvector_64 PC) s.(sregs) = pc) =>
@@ -1863,12 +1863,12 @@ Section UkRunSys.
   Proof.
     intros Hn Hal4.
     iIntros "#Hi Hrun Hsb Hcont".
-    iDestruct "Hrun" as (xi C pt Rfd Rut sz M pm fdv cw gn cs pidv) "(%Hlo & %Hpm & %HRut & Hheap & Hstk & Hufd & Hcwda & Hcha & #Hmy & Hpayv & #Hdep & Hb)".
+    iDestruct "Hrun" as (xi C pt Rfd Rut sz M pm fdv cw gn cs pidv) "(%Hlo & %Hpm & %Hlzf & %HRut & Hheap & Hstk & Hufd & Hcwda & Hcha & #Hmy & Hpayv & #Hdep & Hb)".
     iMod (udepw_mint N m pc _ M pm _ fdv cw gn cs pidv
                 with "Hdep Hmy Hsb Hheap Hufd") as "(Hheap & Hufd & Hdepn)".
     iDestruct (uinstr_is_uk_instr with "Hheap Hi") as %Hui.
     iDestruct (uvb_x0 with "Hb") as "[%Hx0 Hb]".
-    iApply (UkStep.wp_uk_ecall C pt Rfd Rut pm sz Hlo Hpm HRut M m pc fdv cw gn cs pidv Hui
+    iApply (UkStep.wp_uk_ecall C pt Rfd Rut pm sz Hlo Hpm HRut Hlzf M m pc fdv cw gn cs pidv Hui
               (fun (s : mstate)
                    (Hp : register_lookup cur_privilege s.(sregs) = User)
                    (Hc : register_lookup (R_bitvector_64 PC) s.(sregs) = pc) =>
@@ -1999,7 +1999,7 @@ Section UkRunSys.
   Proof.
     intros Hn Hal4.
     iIntros "#Hi Hrun Hcwd Hsb Hcont".
-    iDestruct "Hrun" as (xi C pt Rfd Rut sz M pm fdv cw gn cs pidv) "(%Hlo & %Hpm & %HRut & Hheap & Hstk & Hufd & Hcwda & Hcha & #Hmy & Hpayv & #Hdep & Hb)".
+    iDestruct "Hrun" as (xi C pt Rfd Rut sz M pm fdv cw gn cs pidv) "(%Hlo & %Hpm & %Hlzf & %HRut & Hheap & Hstk & Hufd & Hcwda & Hcha & #Hmy & Hpayv & #Hdep & Hb)".
     (* the whole point of the leaf: the key's cwd IS the one the caller's
        bundle is stated at *)
     iDestruct (ucwd_agree with "Hcwda Hcwd") as %->.
@@ -2007,7 +2007,7 @@ Section UkRunSys.
                 with "Hdep Hmy Hsb Hheap Hufd") as "(Hheap & Hufd & Hdepn)".
     iDestruct (uinstr_is_uk_instr with "Hheap Hi") as %Hui.
     iDestruct (uvb_x0 with "Hb") as "[%Hx0 Hb]".
-    iApply (UkStep.wp_uk_ecall C pt Rfd Rut pm sz Hlo Hpm HRut M m pc fdv c gn cs pidv Hui
+    iApply (UkStep.wp_uk_ecall C pt Rfd Rut pm sz Hlo Hpm HRut Hlzf M m pc fdv c gn cs pidv Hui
               (fun (s : mstate)
                    (Hp : register_lookup cur_privilege s.(sregs) = User)
                    (Hc : register_lookup (R_bitvector_64 PC) s.(sregs) = pc) =>
@@ -2117,12 +2117,12 @@ Section UkRunSys.
   Proof.
     intros Hn Hz Hal4.
     iIntros "#Hi Hrun Hsb Hch Hcont".
-    iDestruct "Hrun" as (xi C pt Rfd Rut sz M pm fdv cw gn cs pidv) "(%Hlo & %Hpm & %HRut & Hheap & Hstk & Hufd & Hcwda & Hcha & #Hmy & Hpayv & #Hdep & Hb)".
+    iDestruct "Hrun" as (xi C pt Rfd Rut sz M pm fdv cw gn cs pidv) "(%Hlo & %Hpm & %Hlzf & %HRut & Hheap & Hstk & Hufd & Hcwda & Hcha & #Hmy & Hpayv & #Hdep & Hb)".
     iMod (udepw_mint N m pc _ M pm _ fdv cw gn cs pidv
                 with "Hdep Hmy Hsb Hheap Hufd") as "(Hheap & Hufd & Hdepn)".
     iDestruct (uinstr_is_uk_instr with "Hheap Hi") as %Hui.
     iDestruct (uvb_x0 with "Hb") as "[%Hx0 Hb]".
-    iApply (UkStep.wp_uk_ecall C pt Rfd Rut pm sz Hlo Hpm HRut M m pc fdv cw gn cs pidv Hui
+    iApply (UkStep.wp_uk_ecall C pt Rfd Rut pm sz Hlo Hpm HRut Hlzf M m pc fdv cw gn cs pidv Hui
               (fun (s : mstate)
                    (Hp : register_lookup cur_privilege s.(sregs) = User)
                    (Hc : register_lookup (R_bitvector_64 PC) s.(sregs) = pc) =>
@@ -2320,7 +2320,7 @@ Section UkRunSys.
   Proof.
     intros Hn Hwin Hcapk Hcl Hdp Hop Hpp Hwt Hal4.
     iIntros "#Hi Hrun Hsb Hbuf Hcont".
-    iDestruct "Hrun" as (xi C pt Rfd Rut sz M pm fdv cw gn cs pidv) "(%Hlo & %Hpm & %HRut & Hheap & Hstk & Hufd & Hcwda & Hcha & #Hmy & Hpayv & #Hdep & Hb)".
+    iDestruct "Hrun" as (xi C pt Rfd Rut sz M pm fdv cw gn cs pidv) "(%Hlo & %Hpm & %Hlzf & %HRut & Hheap & Hstk & Hufd & Hcwda & Hcha & #Hmy & Hpayv & #Hdep & Hb)".
     iMod (udepw_mint N m pc _ M pm _ fdv cw gn cs pidv
                 with "Hdep Hmy Hsb Hheap Hufd") as "(Hheap & Hufd & Hdepn)".
     iDestruct (uinstr_is_uk_instr with "Hheap Hi") as %Hui.
@@ -2334,7 +2334,7 @@ Section UkRunSys.
       change (2 ^ 38) with 274877906944 in Hc.
       rewrite !uint_unsigned in Hc |- *.
       apply uint_add_vec_int_small; lia. }
-    iApply (UkStep.wp_uk_ecall C pt Rfd Rut pm sz Hlo Hpm HRut M m pc fdv cw gn cs pidv Hui
+    iApply (UkStep.wp_uk_ecall C pt Rfd Rut pm sz Hlo Hpm HRut Hlzf M m pc fdv cw gn cs pidv Hui
               (fun (s : mstate)
                    (Hp : register_lookup cur_privilege s.(sregs) = User)
                    (Hc : register_lookup (R_bitvector_64 PC) s.(sregs) = pc) =>
@@ -2430,7 +2430,7 @@ Section UkRunSys.
     (* [uheap_store_run] is a basic update and [ukc] is not a [WP], so the
        re-assembly runs under [ukc]'s own binders -- which is why this leaf
        opens the close by hand instead of applying it to the goal. *)
-    rewrite /ukc. iIntros (h' xi' C' pt' Rfd' Rut') "%Hlo' %Hpm' Hb'".
+    rewrite /ukc. iIntros (h' xi' C' pt' Rfd' Rut') "%Hlo' %Hpm' %Hlzf' Hb'".
     iEval (rewrite (ubytes_split (ukn_d N) (uint dst) d k f Hdk)) in "Hbuf".
     iDestruct "Hbuf" as "[Hblo Hbhi]".
     iMod (uheap_store_run (ukn_t N) (ukn_d N) (ukn_s N) M pm sz (uint dst) d f g with "Hheap Hblo")
@@ -2449,8 +2449,8 @@ Section UkRunSys.
         iApply ("Hcont" $! h'' r d g with "[%] [%] Hrun Hbuf");
         [ exact Hdcap | intros j Hj; apply Hgf; lia ] | ].
     iDestruct (ukcq_ukc with "Hkc") as "Hkc".
-    iApply ("Hkc" $! h' xi' C' pt' Rfd' Rut' with "[%] [%] Hb'");
-      [ exact Hlo' | exact Hpm' ].
+    iApply ("Hkc" $! h' xi' C' pt' Rfd' Rut' with "[%] [%] [%] Hb'");
+      [ exact Hlo' | exact Hpm' | exact Hlzf' ].
   Qed.
 
 
@@ -2522,7 +2522,7 @@ Section UkRunSys.
     intros Hn Hal4.
     set (dst := m !!! Regidx (mword_of_int 10)).
     iIntros "#Hi Hrun Hsb Hstd Hbuf Hcont".
-    iDestruct "Hrun" as (xi C pt Rfd Rut sz M pm fdv cw gn cs pidv) "(%Hlo & %Hpm & %HRut & Hheap & Hstk & Hufd & Hcwda & Hcha & #Hmy & Hpayv & #Hdep & Hb)".
+    iDestruct "Hrun" as (xi C pt Rfd Rut sz M pm fdv cw gn cs pidv) "(%Hlo & %Hpm & %Hlzf & %HRut & Hheap & Hstk & Hufd & Hcwda & Hcha & #Hmy & Hpayv & #Hdep & Hb)".
     iMod (udepw_mint N m pc _ M pm _ fdv cw gn cs pidv
                 with "Hdep Hmy Hsb Hheap Hufd") as "(Hheap & Hufd & Hdepn)".
     iDestruct (uinstr_is_uk_instr with "Hheap Hi") as %Hui.
@@ -2536,7 +2536,7 @@ Section UkRunSys.
       change (2 ^ 38) with 274877906944 in Hc.
       rewrite !uint_unsigned in Hc |- *.
       apply uint_add_vec_int_small; lia. }
-    iApply (UkStep.wp_uk_ecall C pt Rfd Rut pm sz Hlo Hpm HRut M m pc fdv cw gn cs pidv Hui
+    iApply (UkStep.wp_uk_ecall C pt Rfd Rut pm sz Hlo Hpm HRut Hlzf M m pc fdv cw gn cs pidv Hui
               (fun (s : mstate)
                    (Hp : register_lookup cur_privilege s.(sregs) = User)
                    (Hc : register_lookup (R_bitvector_64 PC) s.(sregs) = pc) =>
@@ -2691,7 +2691,7 @@ Section UkRunSys.
     clear HM'. subst M'.
     rewrite (uslot_bump_run m pc M (umem_write M (uint dst) dd gg) pm pm sz sz
                fdv fdv' cw cw' gn gn cs cs pidv false false r Hx0 Hal4).
-    rewrite /ukc. iIntros (h' xi' C' pt' Rfd' Rut') "%Hlo' %Hpm' Hb'".
+    rewrite /ukc. iIntros (h' xi' C' pt' Rfd' Rut') "%Hlo' %Hpm' %Hlzf' Hb'".
     iEval (rewrite (ubytes_split (ukn_d N) (uint dst) dd 8 f Hdd8)) in "Hbuf".
     iDestruct "Hbuf" as "[Hblo Hbhi]".
     iMod (uheap_store_run (ukn_t N) (ukn_d N) (ukn_s N) M pm sz (uint dst) dd f gg with "Hheap Hblo")
@@ -2757,8 +2757,8 @@ Section UkRunSys.
       [ iIntros (h'') "Hrun";
         iApply ("Hcont" $! h'' r gg with "Hhs Hrun Hbuf") | ].
     iDestruct (ukcq_ukc with "Hkc") as "Hkc".
-    iApply ("Hkc" $! h' xi' C' pt' Rfd' Rut' with "[%] [%] Hb'");
-      [ exact Hlo' | exact Hpm' ].
+    iApply ("Hkc" $! h' xi' C' pt' Rfd' Rut' with "[%] [%] [%] Hb'");
+      [ exact Hlo' | exact Hpm' | exact Hlzf' ].
   Qed.
 
   (* ------------------------------------------------------------------- *)
@@ -2965,7 +2965,7 @@ Section UkRunSys.
       destruct (decide (USYS_read = USYS_read)) as [_ | Hc];
         [ | exfalso; exact (Hc eq_refl) ].
       rewrite Hcnt. reflexivity. }
-    iDestruct "Hrun" as (xi C pt Rfd Rut sz M pm fdv cw gn cs pidv) "(%Hlo & %Hpm & %HRut & Hheap & Hstk & Hufd & Hcwda & Hcha & #Hmy & Hpayv & #Hdep & Hb)".
+    iDestruct "Hrun" as (xi C pt Rfd Rut sz M pm fdv cw gn cs pidv) "(%Hlo & %Hpm & %Hlzf & %HRut & Hheap & Hstk & Hufd & Hcwda & Hcha & #Hmy & Hpayv & #Hdep & Hb)".
     (* THE KEY'S LOW THREE SLOTS ARE THE CALLER'S OWN LEDGER, which is both
        what the deposit is stated at and what makes row 5's arm readable *)
     iDestruct (ustd_agree (ukn_fd N) fdv l with "Hufd Hstd") as %Htake.
@@ -2997,7 +2997,7 @@ Section UkRunSys.
       destruct (Hbnd j Hjk) as [_ Hrange].
       apply (UserHeap.lazy_free_uw_addr P sz (uint dst + Z.of_nat j)%Z Hwf Hlf);
         [ exact Hrange | rewrite Hpmp; exact (Hwacc j Hjk) ]. }
-    iApply (UkStep.wp_uk_ecall C pt Rfd Rut pm sz Hlo Hpm HRut M m pc fdv cw gn cs pidv Hui
+    iApply (UkStep.wp_uk_ecall C pt Rfd Rut pm sz Hlo Hpm HRut Hlzf M m pc fdv cw gn cs pidv Hui
               (fun (s : mstate)
                    (Hp : register_lookup cur_privilege s.(sregs) = User)
                    (Hc : register_lookup (R_bitvector_64 PC) s.(sregs) = pc) =>
@@ -3066,7 +3066,7 @@ Section UkRunSys.
     subst fdv'.
     rewrite (uslot_bump_run m pc M (umem_write M (uint dst) d g) pm pm sz sz
                fdv fdv cw cw' gn gn cs cs pidv false false r Hx0 Hal4).
-    rewrite /ukc. iIntros (h' xi' C' pt' Rfd' Rut') "%Hlo' %Hpm' Hb'".
+    rewrite /ukc. iIntros (h' xi' C' pt' Rfd' Rut') "%Hlo' %Hpm' %Hlzf' Hb'".
     iEval (rewrite (ubytes_split (ukn_d N) (uint dst) d k f Hdk)) in "Hbuf".
     iDestruct "Hbuf" as "[Hblo Hbhi]".
     iMod (uheap_store_run (ukn_t N) (ukn_d N) (ukn_s N) M pm sz (uint dst) d f g with "Hheap Hblo")
@@ -3112,8 +3112,8 @@ Section UkRunSys.
       (* definitional: the run is at [false] *)
       - reflexivity. }
     iDestruct (ukcq_ukc with "Hkc") as "Hkc".
-    iApply ("Hkc" $! h' xi' C' pt' Rfd' Rut' with "[%] [%] Hb'");
-      [ exact Hlo' | exact Hpm' ].
+    iApply ("Hkc" $! h' xi' C' pt' Rfd' Rut' with "[%] [%] [%] Hb'");
+      [ exact Hlo' | exact Hpm' | exact Hlzf' ].
   Qed.
 
   (* ------------------------------------------------------------------- *)
@@ -3222,7 +3222,7 @@ Section UkRunSys.
   Proof.
     intros Hn Hal4.
     iIntros "#Hi Hrun Hcwd Hsb Hstd Hcont".
-    iDestruct "Hrun" as (xi C pt Rfd Rut sz M pm fdv cw gn cs pidv) "(%Hlo & %Hpm & %HRut & Hheap & Hstk & Hufd & Hcwda & Hcha & #Hmy & Hpayv & #Hdep & Hb)".
+    iDestruct "Hrun" as (xi C pt Rfd Rut sz M pm fdv cw gn cs pidv) "(%Hlo & %Hpm & %Hlzf & %HRut & Hheap & Hstk & Hufd & Hcwda & Hcha & #Hmy & Hpayv & #Hdep & Hb)".
     (* the key's cwd IS the one the caller's PINNED bundle is stated at *)
     iDestruct (ucwd_agree with "Hcwda Hcwd") as %->.
     (* ...and the key's low three slots ARE the caller's own ledger, which
@@ -3234,7 +3234,7 @@ Section UkRunSys.
       as "(Hheap & Hufd & Hdepn)".
     iDestruct (uinstr_is_uk_instr with "Hheap Hi") as %Hui.
     iDestruct (uvb_x0 with "Hb") as "[%Hx0 Hb]".
-    iApply (UkStep.wp_uk_ecall C pt Rfd Rut pm sz Hlo Hpm HRut M m pc fdv c gn cs pidv Hui
+    iApply (UkStep.wp_uk_ecall C pt Rfd Rut pm sz Hlo Hpm HRut Hlzf M m pc fdv c gn cs pidv Hui
               (fun (s : mstate)
                    (Hp : register_lookup cur_privilege s.(sregs) = User)
                    (Hc : register_lookup (R_bitvector_64 PC) s.(sregs) = pc) =>
@@ -3382,14 +3382,14 @@ Section UkRunSys.
   Proof.
     intros Hn Hexit Hfork Hexec Hsbrk H3 H4 H5 H8 Hcl Hdp Hop Hcd Hal4.
     iIntros "#Hi Hrun Hcwd Hsb Hcont".
-    iDestruct "Hrun" as (xi C pt Rfd Rut sz M pm fdv cw gn cs pidv) "(%Hlo & %Hpm & %HRut & Hheap & Hstk & Hufd & Hcwda & Hcha & #Hmy & Hpayv & #Hdep & Hb)".
+    iDestruct "Hrun" as (xi C pt Rfd Rut sz M pm fdv cw gn cs pidv) "(%Hlo & %Hpm & %Hlzf & %HRut & Hheap & Hstk & Hufd & Hcwda & Hcha & #Hmy & Hpayv & #Hdep & Hb)".
     iDestruct (ucwd_agree with "Hcwda Hcwd") as %->.
     iDestruct "Hsb" as "[%Hfp Hsb]".
     iDestruct ("Hsb" $! M pm sz fdv gn cs pidv with "Hmy Hheap Hufd")
       as "(Hheap & Hufd & Hdepn)".
     iDestruct (uinstr_is_uk_instr with "Hheap Hi") as %Hui.
     iDestruct (uvb_x0 with "Hb") as "[%Hx0 Hb]".
-    iApply (UkStep.wp_uk_ecall C pt Rfd Rut pm sz Hlo Hpm HRut M m pc fdv c gn cs pidv Hui
+    iApply (UkStep.wp_uk_ecall C pt Rfd Rut pm sz Hlo Hpm HRut Hlzf M m pc fdv c gn cs pidv Hui
               (fun (s : mstate)
                    (Hp : register_lookup cur_privilege s.(sregs) = User)
                    (Hc : register_lookup (R_bitvector_64 PC) s.(sregs) = pc) =>
@@ -3520,7 +3520,7 @@ Section UkRunSys.
   Proof.
     intros Hn Hal4.
     iIntros "#Hi #Himg Hrun Hcwd Hsb Hstd Hcont".
-    iDestruct "Hrun" as (xi C pt Rfd Rut sz M pm fdv cw gn cs pidv) "(%Hlo & %Hpm & %HRut & Hheap & Hstk & Hufd & Hcwda & Hcha & #Hmy & Hpayv & #Hdep & Hb)".
+    iDestruct "Hrun" as (xi C pt Rfd Rut sz M pm fdv cw gn cs pidv) "(%Hlo & %Hpm & %Hlzf & %HRut & Hheap & Hstk & Hufd & Hcwda & Hcha & #Hmy & Hpayv & #Hdep & Hb)".
     (* the key's cwd IS the one the caller's PINNED bundle is stated at *)
     iDestruct (ucwd_agree with "Hcwda Hcwd") as %->.
     (* ...and the key's low three slots ARE the caller's own ledger, which
@@ -3541,7 +3541,7 @@ Section UkRunSys.
       as "(Hheap & Hufd & Hdepn)".
     iDestruct (uinstr_is_uk_instr with "Hheap Hi") as %Hui.
     iDestruct (uvb_x0 with "Hb") as "[%Hx0 Hb]".
-    iApply (UkStep.wp_uk_ecall C pt Rfd Rut pm sz Hlo Hpm HRut M m pc fdv c gn cs pidv Hui
+    iApply (UkStep.wp_uk_ecall C pt Rfd Rut pm sz Hlo Hpm HRut Hlzf M m pc fdv c gn cs pidv Hui
               (fun (s : mstate)
                    (Hp : register_lookup cur_privilege s.(sregs) = User)
                    (Hc : register_lookup (R_bitvector_64 PC) s.(sregs) = pc) =>
@@ -3671,7 +3671,7 @@ Section UkRunSys.
   Proof.
     intros Hn Hexit Hfork Hexec Hsbrk H3 H4 H5 H8 Hcl Hdp Hop Hcd Hal4.
     iIntros "#Hi #Himg Hrun Hcwd Hsb Hcont".
-    iDestruct "Hrun" as (xi C pt Rfd Rut sz M pm fdv cw gn cs pidv) "(%Hlo & %Hpm & %HRut & Hheap & Hstk & Hufd & Hcwda & Hcha & #Hmy & Hpayv & #Hdep & Hb)".
+    iDestruct "Hrun" as (xi C pt Rfd Rut sz M pm fdv cw gn cs pidv) "(%Hlo & %Hpm & %Hlzf & %HRut & Hheap & Hstk & Hufd & Hcwda & Hcha & #Hmy & Hpayv & #Hdep & Hb)".
     iDestruct (ucwd_agree with "Hcwda Hcwd") as %->.
     (* ...AND THE IMAGE ROW ([wp_uk_ecall_open_recv_img]'s) *)
     iAssert (⌜ forall (a : Z) (b : bv 8),
@@ -3685,7 +3685,7 @@ Section UkRunSys.
       as "(Hheap & Hufd & Hdepn)".
     iDestruct (uinstr_is_uk_instr with "Hheap Hi") as %Hui.
     iDestruct (uvb_x0 with "Hb") as "[%Hx0 Hb]".
-    iApply (UkStep.wp_uk_ecall C pt Rfd Rut pm sz Hlo Hpm HRut M m pc fdv c gn cs pidv Hui
+    iApply (UkStep.wp_uk_ecall C pt Rfd Rut pm sz Hlo Hpm HRut Hlzf M m pc fdv c gn cs pidv Hui
               (fun (s : mstate)
                    (Hp : register_lookup cur_privilege s.(sregs) = User)
                    (Hc : register_lookup (R_bitvector_64 PC) s.(sregs) = pc) =>
@@ -3841,7 +3841,7 @@ Section UkRunSys.
       change (2 ^ 38)%Z with 274877906944%Z. lia. }
     iIntros "#Hi Hrun Hsb Hsz Hcont".
     iDestruct "Hrun" as (xi C pt Rfd Rut szk M pm fdv cw gn cs pidv)
-      "(%Hlo & %Hpm & %HRut & Hheap & Hstk & Hufd & Hcwda & Hcha & #Hmy & Hpayv & #Hdep & Hb)".
+      "(%Hlo & %Hpm & %Hlzf & %HRut & Hheap & Hstk & Hufd & Hcwda & Hcha & #Hmy & Hpayv & #Hdep & Hb)".
     iMod (udepw_mint N m pc _ M pm _ fdv cw gn cs pidv
                 with "Hdep Hmy Hsb Hheap Hufd") as "(Hheap & Hufd & Hdepn)".
     (* the key's break IS the program's *)
@@ -3870,7 +3870,7 @@ Section UkRunSys.
     iDestruct (UkStep.uvb_pure with "Hb") as "[%Hpure Hb]".
     destruct Hpure as [Mp Hpure].
     iDestruct (uvb_x0 with "Hb") as "[%Hx0 Hb]".
-    iApply (UkStep.wp_uk_ecall C pt Rfd Rut pm sz Hlo Hpm HRut M m pc fdv cw gn cs pidv Hui
+    iApply (UkStep.wp_uk_ecall C pt Rfd Rut pm sz Hlo Hpm HRut Hlzf M m pc fdv cw gn cs pidv Hui
               (fun (s : mstate)
                    (Hp : register_lookup cur_privilege s.(sregs) = User)
                    (Hc : register_lookup (R_bitvector_64 PC) s.(sregs) = pc) =>
@@ -4062,7 +4062,7 @@ Section UkRunSys.
       rewrite Himg.
       rewrite (uslot_bump_run m pc M (umem_grow M (sz + n)) pm pm'
                  sz (sz + n) fdv fdv cw cw' gn gn cs cs pidv false false r Hx0 Hal4).
-      rewrite /ukc. iIntros (h' xi' C' pt' Rfd' Rut') "%Hlo' %Hpm' Hb'".
+      rewrite /ukc. iIntros (h' xi' C' pt' Rfd' Rut') "%Hlo' %Hpm' %Hlzf' Hb'".
       iMod (uheap_grow_run (ukn_t N) (ukn_d N) (ukn_s N) M pm pm' sz n Hsz0 Hn0 Hfresh Hext
               Hcan' Hstop' with "Hheap Hsz") as "(Hheap & Hsz & Hrun')".
       iDestruct (urun_close_upd N (umem_grow M (sz + n)) pm' m
@@ -4073,8 +4073,8 @@ Section UkRunSys.
         iApply ("Hcont" $! h'' r with "[Hsz Hrun'] Hrun").
         iRight. iSplitR; [ iPureIntro; exact Hr | ]. iFrame "Hsz Hrun'". }
       iDestruct (ukcq_ukc with "Hkc") as "Hkc".
-      iApply ("Hkc" $! h' xi' C' pt' Rfd' Rut' with "[%] [%] Hb'");
-        [ exact Hlo' | exact Hpm' ].
+      iApply ("Hkc" $! h' xi' C' pt' Rfd' Rut' with "[%] [%] [%] Hb'");
+        [ exact Hlo' | exact Hpm' | exact Hlzf' ].
   Qed.
 
   (* EXIT PAYS.  The one leaf whose premise is a RESOURCE the program owes
@@ -4102,9 +4102,9 @@ Section UkRunSys.
     WP (Loop : expr riscv_lang).
   Proof.
     intros Hn. iIntros "#Hi Hpay Hrun".
-    iDestruct "Hrun" as (xi C pt Rfd Rut sz M pm fdv cw gn cs pidv) "(%Hlo & %Hpm & %HRut & Hheap & Hstk & Hufd & Hcwda & Hcha & #Hmy & Hpayv & #Hdep & Hb)".
+    iDestruct "Hrun" as (xi C pt Rfd Rut sz M pm fdv cw gn cs pidv) "(%Hlo & %Hpm & %Hlzf & %HRut & Hheap & Hstk & Hufd & Hcwda & Hcha & #Hmy & Hpayv & #Hdep & Hb)".
     iDestruct (uinstr_is_uk_instr with "Hheap Hi") as %Hui.
-    iApply (UkStep.wp_uk_ecall C pt Rfd Rut pm sz Hlo Hpm HRut M m pc fdv cw gn cs pidv Hui
+    iApply (UkStep.wp_uk_ecall C pt Rfd Rut pm sz Hlo Hpm HRut Hlzf M m pc fdv cw gn cs pidv Hui
               (fun (s : mstate)
                    (Hp : register_lookup cur_privilege s.(sregs) = User)
                    (Hc : register_lookup (R_bitvector_64 PC) s.(sregs) = pc) =>
