iris/UkSh.v
@@ -442,7 +442,7 @@ Section UkSh.
     urun N h m pc avail -∗ ubyteq γd dq a b -∗ ⌜ 0 <= a < 2 ^ 38 ⌝.
   Proof.
     iIntros "Hrun Hb".
-    iDestruct "Hrun" as (xi C pt Rfd Rut sz M pm fdv cw gn cs pidv) "(_ & _ & _ & Hh & _ & _ & _ & _)".
+    iDestruct "Hrun" as (xi C pt Rfd Rut sz M pm fdv cw gn cs pidv) "(_ & _ & _ & _ & Hh & _ & _ & _ & _)".
     iDestruct (uheap_ubyte with "Hh Hb") as %(_ & _ & Hbnd).
     iPureIntro. exact Hbnd.
   Qed.
@@ -473,12 +473,12 @@ Section UkSh.
     ⌜ m !!! Regidx x0_idx = zero_reg ⌝ ∗ urun N h m pc avail.
   Proof.
     iIntros "Hrun".
-    iDestruct "Hrun" as (xi C pt Rfd Rut sz M pm fdv cw gn cs pidv) "(%Hlo & %Hpm & %HRut & Hheap & Hstk & Hufd & Hcwda & Hcha & #Hmy & Hpayv & #Hdep & Hb)".
+    iDestruct "Hrun" as (xi C pt Rfd Rut sz M pm fdv cw gn cs pidv) "(%Hlo & %Hpm & %Hlzf & %HRut & Hheap & Hstk & Hufd & Hcwda & Hcha & #Hmy & Hpayv & #Hdep & Hb)".
     iDestruct (uvb_x0 with "Hb") as "[%Hx0 Hb]".
     iSplitR; [ iPureIntro; exact Hx0 | ].
     iExists xi, C, pt, Rfd, Rut, sz, M, pm, fdv, cw, gn, cs, pidv.
     iFrame "Hheap Hstk Hufd Hcwda Hcha Hmy Hpayv Hdep Hb".
-    iPureIntro. split_and!; [ exact Hlo | exact Hpm | exact HRut ].
+    iPureIntro. split_and!; [ exact Hlo | exact Hpm | exact Hlzf | exact HRut ].
   Qed.
 
   Local Lemma ush_nth_byte0_zero : nth_byte (zero_reg : mword 64) 0 = ubyte0.
