iris/UkShRun.v
@@ -502,7 +502,7 @@ Section UkShRun.
     WP (Loop : expr riscv_lang).
   Proof.
     intros Hns He1 He2 Ha Hal Hrd. iIntros "#Hi Hw Hrun Hcont".
-    iDestruct "Hrun" as (xi C pt Rfd Rut sz M pm fdv cw gn cs pidv) "(%Hlo & %Hpm & %HRut & Hheap & Hstk & Hufd & Hcwda & Hcha & #Hmy & Hpayv & #Hdep & Hb)".
+    iDestruct "Hrun" as (xi C pt Rfd Rut sz M pm fdv cw gn cs pidv) "(%Hlo & %Hpm & %Hlzf & %HRut & Hheap & Hstk & Hufd & Hcwda & Hcha & #Hmy & Hpayv & #Hdep & Hb)".
     iDestruct (uinstr_is_uk_instr with "Hheap Hi") as %Hui.
     iDestruct (uheap_access (ukn_t N) (ukn_d N) (ukn_s N) M pm sz dq a 8 (nth_byte w)
                  ltac:(lia) ltac:(right; right; right; reflexivity) Hal
@@ -514,7 +514,7 @@ Section UkShRun.
                           (concat_vec uimm ('b"000"))))).
     { rewrite Ha /uoff_c8. rewrite <- moi_add. rewrite !moi_of_uint.
       reflexivity. }
-    iApply (UkLoad.wp_uk_cld C pt Rfd Rut pm sz Hlo Hpm HRut M m pc fdv cw gn cs pidv uimm crs1 crd rs1 rd
+    iApply (UkLoad.wp_uk_cld C pt Rfd Rut pm sz Hlo Hpm HRut Hlzf M m pc fdv cw gn cs pidv uimm crs1 crd rs1 rd
               (mword_of_int a) w Hui He1 He2 Hrd Htgt
               Hok
               Hcan Hpg Hal8
@@ -545,7 +545,7 @@ Section UkShRun.
     WP (Loop : expr riscv_lang).
   Proof.
     intros Hns He1 He2 Ha Hal Hrd. iIntros "#Hi Hw Hrun Hcont".
-    iDestruct "Hrun" as (xi C pt Rfd Rut sz M pm fdv cw gn cs pidv) "(%Hlo & %Hpm & %HRut & Hheap & Hstk & Hufd & Hcwda & Hcha & #Hmy & Hpayv & #Hdep & Hb)".
+    iDestruct "Hrun" as (xi C pt Rfd Rut sz M pm fdv cw gn cs pidv) "(%Hlo & %Hpm & %Hlzf & %HRut & Hheap & Hstk & Hufd & Hcwda & Hcha & #Hmy & Hpayv & #Hdep & Hb)".
     iDestruct (uinstr_is_uk_instr with "Hheap Hi") as %Hui.
     iDestruct (uheap_access (ukn_t N) (ukn_d N) (ukn_s N) M pm sz dq a 4 (nth_byte wv)
                  ltac:(lia) ltac:(right; right; left; reflexivity) Hal
@@ -557,7 +557,7 @@ Section UkShRun.
                           (concat_vec uimm ('b"00"))))).
     { rewrite Ha /uoff_c4. rewrite <- moi_add. rewrite !moi_of_uint.
       reflexivity. }
-    iApply (UkLoad.wp_uk_clw C pt Rfd Rut pm sz Hlo Hpm HRut M m pc fdv cw gn cs pidv uimm crs1 crd rs1 rd
+    iApply (UkLoad.wp_uk_clw C pt Rfd Rut pm sz Hlo Hpm HRut Hlzf M m pc fdv cw gn cs pidv uimm crs1 crd rs1 rd
               (mword_of_int a) (sign_extend' 64 wv) wv Hui He1 He2 Hrd Htgt
               Hok
               Hcan Hpg Hal8
@@ -586,7 +586,7 @@ Section UkShRun.
     WP (Loop : expr riscv_lang).
   Proof.
     intros Hns Ha Hal Hrd. iIntros "#Hi Hw Hrun Hcont".
-    iDestruct "Hrun" as (xi C pt Rfd Rut sz M pm fdv cw gn cs pidv) "(%Hlo & %Hpm & %HRut & Hheap & Hstk & Hufd & Hcwda & Hcha & #Hmy & Hpayv & #Hdep & Hb)".
+    iDestruct "Hrun" as (xi C pt Rfd Rut sz M pm fdv cw gn cs pidv) "(%Hlo & %Hpm & %Hlzf & %HRut & Hheap & Hstk & Hufd & Hcwda & Hcha & #Hmy & Hpayv & #Hdep & Hb)".
     iDestruct (uinstr_is_uk_instr with "Hheap Hi") as %Hui.
     iDestruct (uheap_access (ukn_t N) (ukn_d N) (ukn_s N) M pm sz dq a 4 (nth_byte wv)
                  ltac:(lia) ltac:(right; right; left; reflexivity) Hal
@@ -595,7 +595,7 @@ Section UkShRun.
     assert (Htgt : (mword_of_int a : mword 64)
                    = add_vec (m !!! Regidx rs1) (sign_extend' 64 imm)).
     { exact (umoi_add_i12 _ imm a Ha). }
-    iApply (UkLoad.wp_uk_lwu C pt Rfd Rut pm sz Hlo Hpm HRut M m pc fdv cw gn cs pidv imm rs1 rd
+    iApply (UkLoad.wp_uk_lwu C pt Rfd Rut pm sz Hlo Hpm HRut Hlzf M m pc fdv cw gn cs pidv imm rs1 rd
               (mword_of_int a) (zero_extend' 64 wv) wv Hui Hrd Htgt
               Hok
               Hcan Hpg Hal8
