iris/UtResFits.v
@@ -21,6 +21,7 @@ Require Import RiscvLang RiscvPtsto.
    do not get auto-generalized (the one-[Require]-isn't-enough trap) *)
 Require Import FdSlots FileInvDefs IrefSlots ProcAvail Xv6Cameras ProcDefs.
 Require Import ProcPtOwn UserPtTree ProcGeom TimerCap.
+Require Import UserPerm.   (* [lazy_free] -- the residue's fill row *)
 Require Import ProcInv.   (* [us_tf] / [us_upt] -- the residue index's updaters *)
 Require Import IntrDefs KptShare.
 Require Import UsertrapRes.
@@ -190,6 +191,13 @@ Module UtResFits (SY : SYSCALL) <: USERTRAP_RES_PARK.
       `{!riscvGS Σ, !xv6G Σ, !bioslotG Σ, !fdslotG Σ, !fileG Σ, !irefslotG Σ, !pavG Σ, !wchG Σ} `{!ufdG Σ} `{GEN : GenId} `{CID : CpuId} `{XI : CurCtx} (pt : uptd) (ksp : mword 64) (U : ustate) (sts : list fdstate) (cs : gset gname) (pid : mword 32) :
     usertrap_res_bare pt ksp U sts cs pid -∗ ⌜uint (pv_sz (us_V U)) <= uvm_maxsz⌝.
   Proof. exact (ut_res_bare_sz (SY.syscall_env) pt ksp U sts cs pid). Qed.
+
+  (* the fill row, off the same residue -- see [SpecUsertrap]'s Parameter *)
+  Lemma usertrap_res_bare_lazy
+      `{!riscvGS Σ, !xv6G Σ, !bioslotG Σ, !fdslotG Σ, !fileG Σ, !irefslotG Σ, !pavG Σ, !wchG Σ} `{!ufdG Σ} `{GEN : GenId} `{CID : CpuId} `{XI : CurCtx} (pt : uptd) (ksp : mword 64) (U : ustate) (sts : list fdstate) (cs : gset gname) (pid : mword 32) :
+    usertrap_res_bare pt ksp U sts cs pid -∗
+    ⌜pv_lazy (us_V U) = false -> lazy_free (ud_um pt) (uint (pv_sz (us_V U)))⌝.
+  Proof. exact (ut_res_bare_lazy (SY.syscall_env) pt ksp U sts cs pid). Qed.
 
   Lemma usertrap_res_tf_csrs_open
       `{!riscvGS Σ, !xv6G Σ, !bioslotG Σ, !fdslotG Σ, !fileG Σ, !irefslotG Σ, !pavG Σ, !wchG Σ} `{!ufdG Σ} `{GEN : GenId} `{CID : CpuId} `{XI : CurCtx} (pt : uptd) (ksp : mword 64) (U : ustate) (sts : list fdstate) (cs : gset gname) (pid : mword 32) :
